src/study/Nemonuri.Study.CSharpSyntaxRewriter2.Modifier/Nemonuri.StratifiedNode.TypeTheory1.fst
@@ -77,6 +77,34 @@ let get_expression_sum_kind (#lv:pos) (sn:node lv{ Expression? (get_kind sn) })
   : Tot expression_sum_kind
   = let Expression v0 = (get_kind sn) in v0
 
+
+let may_have_kind_argument (#lv:pos) (sn:node lv)
+  : Tot bool
+  = (Argument? (get_kind sn)) && 
+    (get_children_length sn = 1) &&
+    (Expression? (get_kind (get_child_at sn 0)))
+
+let may_have_kind_argument_need_to_substitute_expression (#lv:pos) (sn:node lv)
+  : Tot bool
+  = (may_have_kind_argument sn) && (
+      match (get_expression_sum_kind (get_child_at sn 0)) with
+      | Expression_block_containing -> true
+      | Expression_blockless_complex -> true
+      | _ -> false
+    )
+
+let may_have_kind_argument_ready_to_substitute_expression (#lv:pos) (sn:node lv)
+  : Tot bool
+  = (may_have_kind_argument sn) && (
+      let esn = (get_child_at sn 0) in
+      match (get_expression_sum_kind esn) with
+      | Expression_blockless_complex -> true
+      | Expression_block_containing ->
+          (not (exists_in_descendant_or_self esn may_have_kind_argument_need_to_substitute_expression))
+      | _ -> false
+    )
+
+
 let rec has_kind_block (#lv:pos) (sn:node lv)
   : Tot bool (decreases lv)
   = Block? (get_kind sn) &&
@@ -87,7 +115,10 @@ and has_kind_statement (#lv:pos) (sn:node lv)
   = Statement? (get_kind sn) && (
       match (get_statement_sum_kind sn) with
       | Statement_normal -> (for_all_children sn has_kind_argument)
-      | Statement_substituted _ -> (get_children_length sn = 1) && (for_all_children sn has_kind_expression)
+      | Statement_substituted _ -> 
+          (get_children_length sn = 1) && 
+          (has_kind_expression (get_child_at sn 0)) && 
+          (not (exists_in_descendant_or_self sn may_have_kind_argument_need_to_substitute_expression))
     )
 
 and has_kind_argument (#lv:pos) (sn:node lv)
@@ -100,185 +131,16 @@ and has_kind_expression (#lv:pos) (sn:node lv)
   : Tot bool (decreases lv)
   = (Expression? (get_kind sn)) && (
       match (get_expression_sum_kind sn) with
-      | Expression_block_containing -> (get_children_length sn >= 1) && (for_all_children sn has_kind_block)
+      | Expression_block_containing -> 
+          (get_children_length sn >= 1) && 
+          (for_all_children sn has_kind_block)
       | Expression_blockless_simple -> (is_leaf sn)
       | Expression_blockless_complex -> (is_leaf sn)
       | Expression_blockless_substituted _ -> (is_leaf sn)
     )
 
 let has_kind_compilation_unit (#lv:pos) (sn:node lv)
-  : Tot bool (decreases lv)
+  : Tot bool
   = (Compilation_unit? (get_kind sn)) &&
     (for_all_children sn has_kind_block)
 
-
-
-
-
-
-
-
-let has_kind_statement_normal (#lv:pos) (sn:node lv)
-  : Tot bool
-  = (has_kind_statement sn) && (Statement_normal? (get_statement_sum_kind sn))
-
-let has_kind_statement_substituted (#lv:pos) (sn:node lv)
-  : Tot bool
-  = (has_kind_statement sn) && (Statement_substituted? (get_statement_sum_kind sn))
-
-
-
-
-let has_kind_expression_block_containing (#lv:pos) (sn:node lv)
-  : Tot bool
-  = (has_kind_expression sn) && (Expression_block_containing? (get_expression_sum_kind sn))
-
-let has_kind_expression_blockless_simple (#lv:pos) (sn:node lv)
-  : Tot bool
-  = (has_kind_expression sn) && (Expression_blockless_simple? (get_expression_sum_kind sn))
-
-let has_kind_expression_blockless_complex (#lv:pos) (sn:node lv)
-  : Tot bool
-  = (has_kind_expression sn) && (Expression_blockless_complex? (get_expression_sum_kind sn))
-
-let has_kind_expression_blockless_substituted (#lv:pos) (sn:node lv)
-  : Tot bool
-  = (has_kind_expression sn) && (Expression_blockless_substituted? (get_expression_sum_kind sn))
-
-
-let get_substitution_index (#lv:pos) (sn:node lv{ (has_kind_statement_substituted sn) || (has_kind_expression_blockless_substituted sn) })
-  : Tot nat
-  = if (has_kind_statement_substituted sn) then
-      Statement_substituted?.substitution_index (get_statement_sum_kind sn) 
-    else
-      Expression_blockless_substituted?.substitution_index (get_expression_sum_kind sn) 
-
-
-let is_valid_expression_block_containing (#lv:pos) (sn:node lv{ has_kind_expression_block_containing sn })
-  : Tot bool
-  = (get_children_length sn >= 1) &&
-    (for_all_children sn has_kind_block)
-
-let is_valid_expression_blockless_simple (#lv:pos) (sn:node lv{ has_kind_expression_blockless_simple sn })
-  : Tot bool
-  = (is_leaf sn)
-
-let is_valid_expression_blockless_complex (#lv:pos) (sn:node lv{ has_kind_expression_blockless_complex sn })
-  : Tot bool
-  = (is_leaf sn)
-
-let is_valid_expression (#lv:pos) (sn:node lv{ has_kind_expression sn })
-  : Tot bool
-  = if (has_kind_expression_block_containing sn) then (is_valid_expression_block_containing sn)
-    else if (has_kind_expression_blockless_simple sn) then (is_valid_expression_blockless_simple sn)
-    else if (has_kind_expression_blockless_complex sn) then (is_valid_expression_blockless_complex sn)
-    else true
-
-let has_kind_expression_and_valid (#lv:pos) (sn:node lv)
-  : Tot bool
-  = (has_kind_expression sn) && (is_valid_expression sn)
-
-let is_valid_argument (#lv:pos) (sn:node lv{ has_kind_argument sn })
-  : Tot bool
-  = (get_children_length sn = 1) &&
-    (has_kind_expression_and_valid (get_child_at sn 0))
-
-let has_kind_argument_and_valid (#lv:pos) (sn:node lv)
-  : Tot bool
-  = (has_kind_argument sn) && (is_valid_argument sn)
-
-let is_valid_statement_normal (#lv:pos) (sn:node lv{ has_kind_statement_normal sn })
-  : Tot bool
-  = (for_all_children sn has_kind_argument_and_valid)
-
-(*
-let rec is_valid_argument_for_statement_substituted (#lv:pos) (sn:node lv{ has_kind_argument_and_valid sn })
-  : Tot bool
-  = 
-*)
-
-(*
-let rec is_valid_expression_for_statement_substituted (#lv:pos) (sn:node lv{ has_kind_expression_and_valid sn })
-  : Tot bool (decreases lv)
-  = if (has_kind_expression_blockless_simple sn) then false
-    else if (has_kind_expression_blockless_substituted sn) then false
-    else if (has_kind_expression_block_containing sn) then (for_all_children sn is_valid_block_for_statement_substituted)
-
-and is_valid_block_for_statement_substituted (#lv:pos) (sn:node lv{ has_kind_block sn })
-  : Tot bool (decreases lv)
-  = (for_all_children sn has_kind_statement) &&
-    (for_all_children sn is_valid_statement_for_statement_substituted)
-
-and is_valid_statement_for_statement_substituted (#lv:pos) (sn:node lv{ has_kind_statement sn })
-  : Tot bool (decreases lv)
-  = if (has_kind_statement_substituted sn) then 
-*)
-
-
-(*
-let is_valid_statement_substituted (#lv:pos) (sn:node lv{ has_kind_statement_substituted sn })
-  : Tot bool
-  = (get_children_length sn = 1) &&
-*)
-
-(*
-let is_kind_blockless_expression_normal (#lv:pos) (sn:node lv)
-  : Tot bool
-  = (is_kind_blockless_expression sn) && (Blockless_expression_normal? (get_blockless_expression_sum_kind sn))
-
-let is_kind_blockless_expression_complex (#lv:pos) (sn:node lv)
-  : Tot bool
-  = (is_kind_blockless_expression sn) && (Blockless_expression_complex? (get_blockless_expression_sum_kind sn))
-
-let is_kind_blockless_expression_substituted (#lv:pos) (sn:node lv)
-  : Tot bool
-  = (is_kind_blockless_expression sn) && (Blockless_expression_substituted? (get_blockless_expression_sum_kind sn))
-
-let get_var_index (#lv:pos) (sn:node lv{is_kind_blockless_expression_substituted sn})
-  : Tot nat
-  = (Blockless_expression_substituted?.var_index (get_blockless_expression_sum_kind sn))
-
-let is_kind_argument (#lv:pos) (sn:node lv)
-  : Tot bool
-  = (is_branch sn) && (Argument? (get_kind sn))
-
-let get_argument_sum_kind (#lv:pos) (sn:node lv{ is_kind_argument sn })
-  : Tot argument_sum_kind
-  = let Argument v0 = (get_kind sn) in v0
-
-let is_kind_argument_s1 (#lv:pos) (sn:node lv)
-  : Tot bool
-  = (is_kind_argument sn) && 
-    (Argument_s1? (get_argument_sum_kind sn)) &&
-    (get_children_length sn = 1) &&
-    (is_kind_blockless_expression (get_child_at sn 0))
-
-let is_kind_statement (#lv:pos) (sn:node lv)
-  : Tot bool
-  = (Statement? (get_kind sn)) &&
-    (for_all sn.children is_kind_argument)
-
-let is_kind_block (#lv:pos) (sn:node lv)
-  : Tot bool
-  = (Block? (get_kind sn)) &&
-    (for_all sn.children is_kind_statement)
-
-let is_kind_compilation_unit (#lv:pos) (sn:node lv)
-  : Tot bool
-  = (Compilation_unit? (get_kind sn)) &&
-    (for_all sn.children is_kind_block)
-
-let is_kind_argument_s0 (#lv:pos) (sn:node lv)
-  : Tot bool
-  = (is_kind_argument sn) && 
-    (Argument_s0? (get_argument_sum_kind sn)) &&
-    (get_children_length sn >= 1) &&
-    (for_all sn.children is_kind_block)
-
-private let lemma_test
-  (#lv:pos) (sn:node lv{ is_kind_compilation_unit sn && get_children_length sn >= 3 })
-  : Lemma (is_kind_block (get_child_at sn 2))
-  = ()
-*)
-
-//let is_argument_ready_to_be_substituted
